@prefix : <http://pid.geoscience.org.au/def/ont/gapd#> .
@prefix owl: <http://www.w3.org/2002/07/owl#> .
@prefix rdf: <http://www.w3.org/1999/02/22-rdf-syntax-ns#> .
@prefix xml: <http://www.w3.org/XML/1998/namespace> .
@prefix xsd: <http://www.w3.org/2001/XMLSchema#> .
@prefix dcat: <http://www.w3.org/ns/dcat#> .
@prefix rdfs: <http://www.w3.org/2000/01/rdf-schema#> .
@prefix vann: <http://purl.org/vocab/vann/> .
@prefix dcterms: <http://purl.org/dc/terms/> .
@prefix sosa: <http://www.w3.org/ns/sosa/> .
@base <http://pid.geoscience.org.au/def/ont/gapd#> .

<http://pid.geoscience.org.au/def/ont/gapd#> rdf:type owl:Ontology ;
                                              owl:versionIRI <http://pid.geoscience.org.au/def/ont/gapd/0.1> ;
                                              owl:imports <http://www.w3.org/ns/dcat> ,
                                                          <http://purl.org/linked-data/registry> ,
                                                          <http://www.w3.org/ns/sosa/> ,
                                                          <http://www.w3.org/ns/prov> ;
                                              rdfs:isDefinedBy <http://pid.geoscience.org.au/def/ont/gapd> ;
                                              owl:versionInfo 1.0 ;
                                              rdfs:comment "This ontology represents many of the classes of information object that Geoscience Australia (GA) delivers publicly and the relationships between them."@en ;
                                              dcterms:modified "2017-06-04"^^xsd:date ;
                                              dcterms:description "This ontology represents many of the classes of information object that Geoscience Australia (GA) delivers publicly and the relationships between them."@en ;
                                              dcterms:creator "Nicholas Car"@en ;
                                              dcterms:title "GA's Public Data Ontology"@en ;
                                              dcterms:license <https://creativecommons.org/licenses/by/4.0/> ;
                                              rdfs:label "GA's Public Data ontology"@en ;
                                              vann:preferredNamespaceUri "http://pid.geoscience.org.au/def/ont/gapd#"^^xsd:string ;
                                              dcterms:creator <http://orcid.org/0000-0002-8742-7730> ;
                                              rdfs:seeAlso <https://github.com/nicholascar/gapd-o> ;
                                              vann:preferredNamespacePrefix "gapd"@en ;
                                              dcterms:created "2016-12-08"^^xsd:date ;
                                              dcterms:rights "(c) Geoscience Australia 2017"@en .

#################################################################
#    Annotation properties
#################################################################

###  http://purl.org/linked-data/registry#containedItemClass
<http://purl.org/linked-data/registry#containedItemClass> rdf:type owl:AnnotationProperty .


###  http://purl.org/linked-data/registry#subregister
<http://purl.org/linked-data/registry#subregister> rdf:type owl:AnnotationProperty .


#################################################################
#    Object Properties
#################################################################

###  http://pid.geoscience.org.au/def/ont/gapd#operatesOn
:operatesOn rdf:type owl:ObjectProperty ;
            owl:inverseOf dcat:distribution ;
            rdfs:domain :WebService ;
            rdfs:range :Dataset ;
            rdfs:comment """Web Services operate on Dataset(s).

This is a restricted version of the inverse of DCAT's distribution property and is a code list value in ISO19115-3.”””@en ;
            rdfs:label \"operates on\"@en .


###  http://pid.geoscience.org.au/def/ont/gapd#wasGeneratedUsingPlan
:wasGeneratedUsingPlan rdf:type owl:ObjectProperty ;
                   rdfs:subPropertyOf :wasDerivedFrom ;
                   rdfs:domain :Dataset ;
                   rdfs:range [ rdf:type owl:Class ;
                                owl:unionOf ( :Plan
                                              :SoftwareRepository
                                            )
                              ] ;
                   rdfs:comment “””Entities may have been generated from Plans (instructions or code). 

Use of this property as per :DatasetX wasGeneratedUsingPlan :PlanY is equivalent to declaring:

:DatasetX a prov:Entity ;
  prov:wasGeneratedBy [
    a prov:Activity [
      prov:qualifiedAssociation [
        prov:Association [
          prov:hadPlan :PlanY ]]] ."""@en .


###  http://www.w3.org/ns/dcat#distribution

#################################################################
#    Classes
#################################################################

###  http://pid.geoscience.org.au/def/ont/gapd#Collection
:Collection rdf:type owl:Class .


###  http://pid.geoscience.org.au/def/ont/gapd#Dataset
:Dataset rdf:type owl:Class ;
         rdfs:subClassOf dcat:Dataset ,
                         <http://www.w3.org/ns/prov#Entity> .


###  http://pid.geoscience.org.au/def/ont/gapd#Plan
:Plan rdf:type owl:Class .


###  http://pid.geoscience.org.au/def/ont/gapd#SoftwareRepository
:SoftwareRepository rdf:type owl:Class ;
                    rdfs:subClassOf :Dataset ;
                    rdfs:comment """A Software Repository is a system such as GitHub or BitBucket that stores and manages software code. 

A Software Repository is also a type of dataset therefor GA's Software Repositories are catalogued in one of GA's catalogues, just as all datasets are."""@en ;
                    rdfs:label "Software Repository"@en .


###  http://pid.geoscience.org.au/def/ont/gapd#WebService
:WebService rdf:type owl:Class ;
            rdfs:subClassOf dcat:Distribution ;
            rdfs:comment "GA's Web Services are a specialised type of a dataset distribution: they are a services that allow for dataset subsetting (querying) and supersetting (merging data from multiple datasets). GA has an extensive catalogue of Open Geospatial Consortium web services but also has a few non-OGC web services, such as bespoke RESTful APIs, database XML APIs and SPARQL endpoints."@en ;
            rdfs:label "Web Service"@en .


###  http://purl.org/vocommons/voaf#Vocabulary
<http://purl.org/vocommons/voaf#Vocabulary> rdfs:subClassOf :Dataset ,
                                                            <http://www.w3.org/2004/02/skos/core#ConceptScheme> .


###  http://www.w3.org/ns/prov#Entity
<http://www.w3.org/ns/prov#Entity> rdf:type owl:Class .


#################################################################
#    Individuals
#################################################################

###  http://pid.geoscience.org.au/def/ont/gapd#Dataset
:Dataset rdf:type owl:NamedIndividual .


###  http://pid.geoscience.org.au/def/ont/gapd#DatasetRegister
:DatasetRegister rdf:type owl:NamedIndividual ,
                          <http://purl.org/linked-data/registry#FederatedRegister> ;
                 <http://purl.org/linked-data/registry#containedItemClass> :Dataset ;
                 <http://purl.org/linked-data/registry#subregister> :OntologyRegister ,
                                                                    :VocabularyRegister ,
                                                                    :eCatDatasetRegister ;
                 rdfs:comment "The conceptual register of all Dataset class objects in GA"@en ;
                 rdfs:label "Dataset Register"@en .


###  http://pid.geoscience.org.au/def/ont/gapd#OntologyRegister
<http://pid.geoscience.org.au/def/ont/> rdf:type owl:NamedIndividual ,
                           <http://purl.org/linked-data/registry#Register> ;
                  <http://purl.org/linked-data/registry#containedItemClass> owl:Ontology ;
                  rdfs:comment "The Register of all of GA's Ontologies"@en ;
                  rdfs:label "Ontology Register"@en .


###  http://pid.geoscience.org.au/def/ont/gapd#SampleRegister
<http://pid.geoscience.org.au/samples/> rdf:type owl:NamedIndividual ,
                         <http://purl.org/linked-data/registry#Register> ;
		<http://purl.org/linked-data/registry#containedItemClass> sosa:Sample ;
                rdfs:comment "The Register of all of GA's Samples. This Register is a web-exposed, multiple ontology-supporting API, using the contents of GA's enterprise database, from multiple schema, aggregated in a Samples table."@en ;
                rdfs:label "Sample Register"@en .


###  http://pid.geoscience.org.au/def/ont/gapd#VocabularyRegister
<http://pid.geoscience.org.au/def/voc/> rdf:type owl:NamedIndividual ,
                             <http://purl.org/linked-data/registry#Register> ;
                    <http://purl.org/linked-data/registry#containedItemClass> <http://purl.org/vocommons/voaf#Vocabulary> ;
                    rdfs:comment "The Register of all of GA's Vocabularies"@en ;
                    rdfs:label "Vocabulary Register"@en .


###  http://pid.geoscience.org.au/def/ont/gapd#eCatDatasetRegister
<http://pid.geoscience.org.au/dataset/> rdf:type owl:NamedIndividual ,
                              <http://purl.org/linked-data/registry#Register> ;
                     <http://purl.org/linked-data/registry#containedItemClass> :Dataset ;
                     rdfs:comment "The Datasets register within eCat, the enterprise catalogue"@en ;
                     rdfs:label "eCat Dataset Register"@en .


###  http://pid.geoscience.org.au/def/ont/gapd#eCatServiceRegister
<http://pid.geoscience.org.au/service/> rdf:type owl:NamedIndividual ,
                              <http://purl.org/linked-data/registry#Register> ;
                     <http://purl.org/linked-data/registry#containedItemClass> :WebService ;
                     rdfs:comment "The Services register within eCat, the enterprise catalogue"@en ;
                     rdfs:label "eCat Services Register"@en .


#################################################################
#    Annotations
#################################################################

:Dataset rdfs:label "Dataset"@en ;
         rdfs:comment "GA's Datasets are both DCAT Datasets and also PROV Entities. This means they have metadata according to DCAT and relations to other Datasets, Agents and Activities according to PROV."@en .


<http://purl.org/vocommons/voaf#Vocabulary> rdfs:comment "A Vocabulary, as published by GA, is both a SKOS ConceptScheme and also a DCAT Dataset. This means its content is in accordance with SKOS but its metadata is in accordance with DCAT."@en ;
                                            rdfs:label "Vocabulary"@en .


###  Generated by the OWL API (version 4.2.8.20170104-2310) https://github.com/owlcs/owlapi
